Gates.v
@@ -3,27 +3,30 @@ Require Export ZX.
 
 Definition ZX_H := 
     (Compose 
-        (@Z_Spider 1 1 (PI/2)) 
+        (Z_Spider 1 1 (PI/2)) 
         (Compose 
-            (@X_Spider 1 1(PI/2)) 
-            (@Z_Spider 1 1 (PI/2)))).
+            (X_Spider 1 1(PI/2)) 
+            (Z_Spider 1 1 (PI/2)))).
 
 Definition ZX_CNOT_l : ZX 2 2 := 
     (Compose 
         (Stack 
-            (@Z_Spider 1 2 0%R) 
+            (Z_Spider 1 2 0%R) 
             Wire) 
         (Stack 
             Wire 
-            (@X_Spider 2 1 0%R))).
+            (X_Spider 2 1 0%R))).
 
 Definition ZX_CNOT_r : ZX 2 2 := 
     (Compose 
         (Stack 
             Wire 
-            (@X_Spider 1 2 0%R))
+            (X_Spider 1 2 0%R))
         (Stack 
-            (@Z_Spider 2 1 0%R) 
+            (Z_Spider 2 1 0%R) 
             Wire)).
+
+Definition ZX_S : ZX 1 1 := Z_Spider 1 1 (PI / 2).
+Definition ZX_T : ZX 1 1 := Z_Spider 1 1 (PI / 4).
 
 Notation ZX_CNOT := ZX_CNOT_l.
