Rules.v
@@ -3,7 +3,7 @@ Require Export ZX.
 Require Export Gates.
 Require Export GateRules.
 
-Lemma Z_0_eq_X_0 : ZX_semantics (@Z_Spider 1 1 0) = ZX_semantics (@X_Spider 1 1 0).
+Lemma Z_0_eq_X_0 : ZX_semantics (Z_Spider 1 1 0) = ZX_semantics (X_Spider 1 1 0).
 Proof.
   simpl.
   unfold Spider_Semantics_Impl; unfold bra_ket_MN.
@@ -13,20 +13,23 @@ Proof.
   solve_matrix.
 Qed.
 
-Theorem identity_removal_Z : ZX_semantics (@Z_Spider 1 1 0) = ZX_semantics Wire.
+Theorem identity_removal_Z : ZX_semantics (Z_Spider 1 1 0) = ZX_semantics Wire.
 Proof.
   reflexivity.
 Qed.
 
-Theorem identity_removal_X : ZX_semantics (@X_Spider 1 1 0) = ZX_semantics Wire.
+Theorem identity_removal_X : ZX_semantics (X_Spider 1 1 0) = ZX_semantics Wire.
 Proof.
   rewrite <- Z_0_eq_X_0.
   reflexivity.
 Qed.
+
+Theorem inverse_Z_Spider : forall nIn nOut α, ZX_semantics (Z_Spider nIn nOut α) = (ZX_semantics (Z_Spider nIn nOut α))†.
+Abort.
 
 Theorem Z_to_X_with_H_Outputs : forall n m α, ZX_semantics (@Z_Spider n (m * 1) α) = ZX_semantics (Compose (@X_Spider n (m * 1) α) (nStack ZX_H m)).
 Proof.
   intro n.
   induction n; intro m; induction m; intros.
   - simpl; unfold Spider_Semantics_Impl; unfold bra_ket_MN; solve_matrix.
-Admitted.
+Abort.
